doc/coq/playground/Var.v
@@ -15,11 +15,9 @@ Section Filter.
   Universe filter_u.
   Inductive filter : tyenv -> assign -> tyenv -> Type@{filter_u} :=
   | Filter_nil : filter [] [] []
-  | Filter_cons_some A a γ σ γ'
-    (FILTER : filter γ σ γ')
+  | Filter_cons_some A a γ σ γ' (FILTER : filter γ σ γ')
     : filter (A :: γ) (existT option A (Some a) :: σ) γ'
-  | Filter_cons_none A γ σ γ'
-    (FILTER : filter γ σ γ')
+  | Filter_cons_none A γ σ γ' (FILTER : filter γ σ γ')
     : filter (A :: γ) (existT option A None :: σ) (A :: γ')
   .
 End Filter.
@@ -56,26 +54,47 @@ Proof.
   end).
 Defined.
 
+Definition lift_var Γ : forall {A γ}, var γ A -> var (γ ++ Γ) A :=
+  fix go {A γ} x :=
+  match γ return var γ A -> var (γ ++ Γ) A with
+  | [] => empty_var
+  | τ :: τl => fun x =>
+    match x in var Aγ B return
+      match Aγ with
+      | [] => unit
+      | A :: γ => var (A :: γ ++ Γ) B
+      end
+    with
+    | Var_hd => Var_hd
+    | Var_tl x => Var_tl (go x)
+    end
+  end x.
+
+Definition lift_value Γ {A γ} (v : value γ A) : value (γ ++ Γ) A :=
+  match v with
+  | Var x => Var (lift_var Γ x)
+  | Val v => Val v
+  end.
+
+Definition shift_var {γ A} B (x : var γ A) : var (B :: γ) A :=
+  match γ return var γ A -> var (B :: γ) A with
+  | [] => empty_var
+  | τ :: τl => fun x =>
+    match x in var γ' A
+      return
+        match γ' with
+        | [] => unit
+        | _ :: _ => var (B :: γ') A
+        end
+    with
+    | Var_hd => Var_tl Var_hd
+    | Var_tl x => Var_tl (Var_tl x)
+    end
+  end x.
+
 Definition shift_value {γ A} B (v : value γ A) : value (B :: γ) A :=
   match v in value _ A return value (B :: γ) A with
-  | @Var _ A x =>
-    let convoy A (x : var γ A) :=
-      match γ as γ' return var γ' A -> value (B :: γ') A with
-      | [] => empty_var
-      | τ :: τl => fun x =>
-        match x in var γ' A
-          return
-            match γ' return Type with
-            | [] => unit
-            | _ :: _ => value (B :: γ') A
-            end
-        with
-        | Var_hd => Var (Var_tl Var_hd)
-        | Var_tl x => Var (Var_tl (Var_tl x))
-        end
-      end x
-    in
-    convoy A x
+  | Var x => Var (shift_var B x)
   | Val v => Val v
   end.
 
@@ -122,6 +141,16 @@ Definition assign_value {A} γ σ γ'
   | @Var _ τ x => assign_var γ σ γ' FILTER x
   | @Val _ τ v' => Val v'
   end.
+
+Lemma shift_assign γ σ γ' (FILTER : filter γ σ γ')
+  : forall A B (v : value γ A),
+      shift_value B (assign_value γ σ γ' FILTER v) =
+      assign_value (B :: γ) (existT option B None :: σ) (B :: γ') (Filter_cons_none _ _ _ _ FILTER) (shift_value B v).
+Proof.
+  do 3 intro; destruct v.
+  - destruct x; reflexivity.
+  - reflexivity.
+Qed.
 
 Fixpoint id_filter γ : {σ & filter γ σ γ} :=
   match γ with
